@prefix rdf: <http://www.w3.org/1999/02/22-rdf-syntax-ns#> .

<http://purl.org/coar/version>
    a <http://www.w3.org/2004/02/skos/core#ConceptScheme> .

<http://purl.org/coar/version/c_71e4c1898caa6e32>
    <http://purl.org/dc/terms/modified> "2019-04-17T21:29:35Z"^^<http://www.w3.org/2001/XMLSchema#dateTime> ;
    a <http://www.w3.org/2004/02/skos/core#Concept> ;
    <http://www.w3.org/2004/02/skos/core#altLabel> "preprint"@es, "preprint"@fr, "preprint"@nl, "prépublication"@fr, "submitted manuscript under review"@en, "submitted version"@en, "versión enviada a revisión"@es, "versión enviada a revisión por pares"@es, "versión enviada al editor"@es, "versión no evaluada por pares"@es, "на рассмотрении в редакции"@ru, "на рассмотрении журнала"@ru, "рукопись принятая к рассмотрению"@ru ;
    <http://www.w3.org/2004/02/skos/core#definition> """Any version of a resource that is under formal review managed by a socially recognized publishing entity. The entity recognizes its responsibility to provide objective expert review and feedback to the author, and, ultimately, to pass judgment on the fitness of the resource for publication with an “accept” or “reject” decision. May have a version number or date stamp. Content and layout follow publisher’s submission requirements.
(adapted from NISO-JAV, https://www.niso.org/publications/niso-rp-8-2008-jav)
"""@en ;
    <http://www.w3.org/2004/02/skos/core#exactMatch> <http://purl.org/info:eu-repo/semantics/submittedVersion> ;
    <http://www.w3.org/2004/02/skos/core#inScheme> <http://purl.org/coar/version> ;
    <http://www.w3.org/2004/02/skos/core#prefLabel> "Hakem değerlendirmesi için gönderilmiş versiyon"@tr, "SMUR"@en, "eingereichte Version"@de, "ingediende versie"@nl, "version soumise"@fr, "versione sottoposta a revisione"@it, "versión sometida a revisión"@es, "на рассмотрении на предмет публикации"@ru, "査読版"@ja ;
    <http://www.w3.org/2004/02/skos/core#topConceptOf> <http://purl.org/coar/version> .

<http://purl.org/coar/version/c_970fb48d4fbd8a85>
    <http://purl.org/dc/terms/modified> "2019-04-17T21:29:34Z"^^<http://www.w3.org/2001/XMLSchema#dateTime> ;
    a <http://www.w3.org/2004/02/skos/core#Concept> ;
    <http://www.w3.org/2004/02/skos/core#altLabel> "originale Verlagspublikation"@de, "publisher version"@en, "reprint"@fr, "versie"@nl, "version finale"@fr, "version of record"@en, "version éditée"@fr, "versión final del editor"@es, "версия данных"@ru, "версия записи"@ru ;
    <http://www.w3.org/2004/02/skos/core#definition> """A fixed version of a resource that has been made available by any organization that acts as a publisher by formally and exclusively declaring the resource “published”. This includes any “early release” resource that is formally identified as being published even before the compilation of a volume issue and assignment of associated metadata, as long as it is citable via some permanent identifier(s). This does not include any “early release” resource that has not yet been “fixed” by processes that are still to be applied, such as copy-editing, proof corrections, layout, and typesetting.
(adapted from NISO-JAV, https://www.niso.org/publications/niso-rp-8-2008-jav)
"""@en ;
    <http://www.w3.org/2004/02/skos/core#exactMatch> <http://purl.org/info:eu-repo/semantics/publishedVersion> ;
    <http://www.w3.org/2004/02/skos/core#inScheme> <http://purl.org/coar/version> ;
    <http://www.w3.org/2004/02/skos/core#prefLabel> "Erstpublikation"@de, "VoR"@en, "Yayıncı versiyonu"@tr, "gepubliceerde versie"@nl, "version publiée"@fr, "versione pubblicata"@it, "versión publicada"@es, "версия публикации"@ru, "出版社版"@ja ;
    <http://www.w3.org/2004/02/skos/core#topConceptOf> <http://purl.org/coar/version> .

<http://purl.org/coar/version/c_ab4af688f83e57aa>
    <http://purl.org/dc/terms/modified> "2019-04-17T21:29:34Z"^^<http://www.w3.org/2001/XMLSchema#dateTime> ;
    a <http://www.w3.org/2004/02/skos/core#Concept> ;
    <http://www.w3.org/2004/02/skos/core#altLabel> "Post-Print"@de, "accepted manuscript"@en, "accepted version"@en, "manuscrito aceptado"@es, "postprint"@es, "postprint"@fr, "postprint version"@en, "postpublication"@fr, "versión aceptada para publicar"@es, "материалы принятые к публикации "@ru, "принятая к публикации рукопись"@ru, "рукопись принятая к публикации"@ru, "статья принятая к публикации"@ru ;
    <http://www.w3.org/2004/02/skos/core#definition> """The version of a resource that has been accepted for publication. A second party takes permanent responsibility for the resource. Content and layout follow publisher’s submission requirements.
(adapted from NISO-JAV, https://www.niso.org/publications/niso-rp-8-2008-jav)"""@en ;
    <http://www.w3.org/2004/02/skos/core#exactMatch> <http://purl.org/info:eu-repo/semantics/acceptedVersion> ;
    <http://www.w3.org/2004/02/skos/core#inScheme> <http://purl.org/coar/version> ;
    <http://www.w3.org/2004/02/skos/core#prefLabel> "AM"@en, "Yayına kabul edilmiş versiyon"@tr, "akzeptiertes Manuskript"@de, "geaccepteerde versie"@nl, "version acceptée"@fr, "versione accettata per la pubblicazione"@it, "versión final del autor"@es, "материал принятый к публикации "@ru, "出版社受理版"@ja ;
    <http://www.w3.org/2004/02/skos/core#topConceptOf> <http://purl.org/coar/version> .

<http://purl.org/coar/version/c_b1a7d7d4d402bcce>
    <http://purl.org/dc/terms/modified> "2019-04-17T21:29:34Z"^^<http://www.w3.org/2001/XMLSchema#dateTime> ;
    a <http://www.w3.org/2004/02/skos/core#Concept> ;
    <http://www.w3.org/2004/02/skos/core#altLabel> "author's original"@en, "borrador"@es, "draft"@en, "manuscrito"@es, "première version"@fr, "preprint version"@en, "version d'origine"@fr, "Ön baskı"@tr, "оригинал"@ru ;
    <http://www.w3.org/2004/02/skos/core#definition> """Any version of a resource that is considered by the author to be of sufficient quality to be submitted for formal peer review by a second party. The author accepts full responsibility for the resource . May have a version number or date stamp. Content and layout as set out by the author.
(adapted from NISO-JAV, https://www.niso.org/publications/niso-rp-8-2008-jav)"""@en ;
    <http://www.w3.org/2004/02/skos/core#exactMatch> <http://purl.org/info:eu-repo/semantics/authorVersion> ;
    <http://www.w3.org/2004/02/skos/core#inScheme> <http://purl.org/coar/version> ;
    <http://www.w3.org/2004/02/skos/core#prefLabel> "AO"@en, "Autorenversion"@de, "Yazarın orijinal versiyonu"@tr, "auteurs versie"@nl, "version originale"@fr, "versione originale dell'autore"@it, "versión original del autor"@es, "авторский оригинал"@ru, "著者オリジナル版"@ja ;
    <http://www.w3.org/2004/02/skos/core#topConceptOf> <http://purl.org/coar/version> .

<http://purl.org/coar/version/c_be7fb7dd8ff6fe43>
    <http://purl.org/dc/terms/modified> "2019-04-17T21:29:34Z"^^<http://www.w3.org/2001/XMLSchema#dateTime> ;
    a <http://www.w3.org/2004/02/skos/core#Concept> ;
    <http://www.w3.org/2004/02/skos/core#altLabel> "autre version"@fr, "no aplica"@es, "non applicabile (o ignoto)"@it, "not applicable (or unknown)"@en, "otros"@es ;
    <http://www.w3.org/2004/02/skos/core#definition> "Not Applicable	(or Unknown)"@en ;
    <http://www.w3.org/2004/02/skos/core#inScheme> <http://purl.org/coar/version> ;
    <http://www.w3.org/2004/02/skos/core#prefLabel> "NA"@en, "Uygulanabilir değil"@tr, "keine Angabe"@de, "niet van toepassing (onbekend)"@nl, "non applicabile"@it, "versión desconocida"@es, "не применимо (или неизвестно)"@ru, "適用外"@ja ;
    <http://www.w3.org/2004/02/skos/core#topConceptOf> <http://purl.org/coar/version> .

<http://purl.org/coar/version/c_dc82b40f9837b551>
    <http://purl.org/dc/terms/modified> "2019-04-17T21:29:35Z"^^<http://www.w3.org/2001/XMLSchema#dateTime> ;
    a <http://www.w3.org/2004/02/skos/core#Concept> ;
    <http://www.w3.org/2004/02/skos/core#altLabel> "aktualisierte Version"@de, "enhanced version of record"@en, "gewijzigde versie"@nl, "version amendée"@fr ;
    <http://www.w3.org/2004/02/skos/core#definition> """A version of the Version of Record of a resource that has been updated or 
enhanced by the provision of supplementary material.
(adapted from NISO-JAV, https://www.niso.org/publications/niso-rp-8-2008-jav)
"""@en ;
    <http://www.w3.org/2004/02/skos/core#exactMatch> <http://purl.org/info:eu-repo/semantics/updatedVersion> ;
    <http://www.w3.org/2004/02/skos/core#inScheme> <http://purl.org/coar/version> ;
    <http://www.w3.org/2004/02/skos/core#prefLabel> "EVoR"@en, "Eserin geliştirilmiş versiyonu"@tr, "erweiterte Version"@de, "revisie"@nl, "version améliorée"@fr, "versione revisionata"@it, "versión mejorada"@es, "расширенная версия"@ru, "更新版"@ja ;
    <http://www.w3.org/2004/02/skos/core#topConceptOf> <http://purl.org/coar/version> .

<http://purl.org/coar/version/c_e19f295774971610>
    <http://purl.org/dc/terms/modified> "2019-04-17T21:29:34Z"^^<http://www.w3.org/2001/XMLSchema#dateTime> ;
    a <http://www.w3.org/2004/02/skos/core#Concept> ;
    <http://www.w3.org/2004/02/skos/core#altLabel> "corrected version of record"@en, "gecorrigeerde versie"@nl, "versión publicada corregida"@es ;
    <http://www.w3.org/2004/02/skos/core#definition> """A version of the Version of Record of a resource in which errors in the VoR have been corrected. The errors may be author errors, publisher errors, or other processing errors.
(adapted from NISO-JAV, https://www.niso.org/publications/niso-rp-8-2008-jav)
"""@en ;
    <http://www.w3.org/2004/02/skos/core#exactMatch> <http://purl.org/info:eu-repo/semantics/updatedVersion> ;
    <http://www.w3.org/2004/02/skos/core#inScheme> <http://purl.org/coar/version> ;
    <http://www.w3.org/2004/02/skos/core#prefLabel> "CVoR"@en, "Eserin düzeltilmiş versiyonu"@tr, "herziene versie"@nl, "korrigierte Version"@de, "version corrigée"@fr, "versione corretta"@it, "versión corregida"@es, "исправленная версия "@ru, "訂正版"@ja ;
    <http://www.w3.org/2004/02/skos/core#topConceptOf> <http://purl.org/coar/version> .

<http://purl.org/coar/version/c_fa2ee174bc00049f>
    <http://purl.org/dc/terms/modified> "2019-04-17T21:29:34Z"^^<http://www.w3.org/2001/XMLSchema#dateTime> ;
    a <http://www.w3.org/2004/02/skos/core#Concept> ;
    <http://www.w3.org/2004/02/skos/core#altLabel> "Yayıncı tarafından düzenlenmiş versiyon"@tr, "drukproef"@nl, "manuscrito aceptado"@es, "manuscrito editado"@es, "proof"@en, "version"@fr, "одобрена"@ru, "одобренная"@ru, "одобренные"@ru, "одобренный"@ru, "одобрено"@ru, "одобрены"@ru ;
    <http://www.w3.org/2004/02/skos/core#definition> """A version of a resource that is created as part of the publication process. This includes the copy-edited manuscript, galley proofs (i.e., a typeset version that has not been made up into pages), page proofs, and revised proofs. Some of these versions may remain essentially internal process versions, but others are commonly released from the internal environment (e.g., proofs are sent to authors) and may thus become public, even though they are not authorized to be so. Content has been changed from Accepted Manuscript; layout is the publisher’s.
(adapted from NISO-JAV, https://www.niso.org/publications/niso-rp-8-2008-jav)
"""@en ;
    <http://www.w3.org/2004/02/skos/core#inScheme> <http://purl.org/coar/version> ;
    <http://www.w3.org/2004/02/skos/core#prefLabel> "Korrekturfahne"@de, "P"@en, "Redakte edilmiş versiyon"@tr, "bozza"@it, "proefdruk"@nl, "prueba de galera"@es, "одобрен"@ru, "校正版"@ja ;
    <http://www.w3.org/2004/02/skos/core#topConceptOf> <http://purl.org/coar/version> .
